\documentclass{report}
\usepackage{amsmath}

\newcommand\ddfrac[2]{\frac{\displaystyle #1}{\displaystyle #2}}

\begin{document}
$\theta_r + d\theta_r$\\
$\theta_t + d\theta_t$\\
$dx$\\
$R$\\
$$ \vec{\nabla} \cdot \vec{E} = 4\pi\rho $$
$$ \vec{\nabla} \cdot \vec{B} = 0 $$
$$ \vec{\nabla} \times \vec{E} = -\ddfrac{1}{c}\ddfrac{\partial\vec{B}}{\partial{t}}$$
$$ \vec{\nabla} \times \vec{B} = \ddfrac{4\pi}{c}\vec{J} + \ddfrac{1}{c}\ddfrac{\partial\vec{E}}{\partial{t}} $$

$$ \vec{E}(x,t) = \vec{E}(x)e^{-\kappa z}\cos(kx-\omega t)$$

$$ \kappa = \ddfrac{\omega}{c}\sqrt{\left(n_i\sin\theta_i\right)^2-n_t^2} $$

$$ n_i > n_t $$

\end{document}
